<div class="alert alert-warning" role="alert">
<h4 class="alert-heading">Problem 1</h4>

Use the Laws of Exponents to rewrite and simplify each expression.

1. $\displaystyle \frac{-2^6}{4^3}$

2. $\displaystyle \frac{(-3)^6}{9^6}$

3. $\displaystyle \frac{1}{\sqrt[4]{x^5}}$

4. $\displaystyle \frac{x^3 \cdot x^n}{x^{n+1}}$

5. $\displaystyle b^3(3b^{-1})^{-2}$

6. $\displaystyle \frac{2x^2y}{(3x^{-2}y)^2}$

</div>

<div class="alert alert-success" role="alert">
<h4 class="alert-heading">Solution</h4>

1. $\displaystyle \frac{-2^6}{4^3} = -\frac{2^6}{(2^2)^3} = -\frac{2^6}{2^6} = -1$

2. $\displaystyle \frac{(-3)^6}{9^6} = \frac{3^6}{(3^2)^6} = \frac{3^6}{3^{12}} = 3^{-6}$

3. $\displaystyle \frac{1}{\sqrt[4]{x^5}} = \frac{1}{\sqrt[4]{x^4 \cdot x}} = \frac{1}{x\sqrt[4]{x}}$

4. $\displaystyle \frac{x^3 \cdot x^n}{x^{n+1}} = \frac{x^{n+3}}{x^{n+1}} = x^2$

5. $\displaystyle b^3(3b^{-1})^{-2} = b^3 \cdot 3^{-2} \cdot b^2 = 3^{-2}b^5 = \frac{b^5}{9}$

6. $\displaystyle \frac{2x^2y}{(3x^{-2}y)^2} = \frac{2x^2y}{9x^{-4}y^2} = \frac{2}{9} \cdot \frac{x^2}{x^{-4}} \cdot \frac{y}{y^2} = \frac{2}{9} \cdot x^6 \cdot \frac{1}{y} = \frac{2x^6}{9y}$

</div>
