<div class="alert alert-warning" role="alert">
<h4 class="alert-heading">Problem 2</h4>

Use the Laws of Exponents to rewrite and simplify each expression.

1. $\displaystyle \frac{\sqrt[3]{4}}{\sqrt[3]{108}}$

2. $\displaystyle 27^{2/3}$

3. $\displaystyle 2x^2(3x^5)^2$

4. $\displaystyle (2x^{-2})^{-3}x^{-3}$

5. $\displaystyle \frac{3a^{3/2} \cdot a^{1/2}}{a^{-1}}$

6. $\displaystyle \frac{\sqrt{a\sqrt{b}}}{\sqrt[3]{ab}}$

</div>

<div class="alert alert-success" role="alert">
<h4 class="alert-heading">Solution</h4>

1. $\displaystyle \frac{\sqrt[3]{4}}{\sqrt[3]{108}} = \sqrt[3]{\frac{4}{108}} = \sqrt[3]{\frac{1}{27}} = \frac{1}{\sqrt[3]{3^3}} = \frac{1}{3}$

2. $\displaystyle 27^{2/3} = (3^3)^{\frac{2}{3}} = 3^{(3 \times \frac{2}{3})} = 3^2 = 9$

3. $\displaystyle 2x^2(3x^5)^2 = 2x^2 \cdot 9x^{10} = 18x^{(2+10)} = 18x^{12}$

4. $\displaystyle (2x^{-2})^{-3}x^{-3} = 2^{-3} \cdot x^6 \cdot x^{-3} = \frac{x^{(6-3)}}{2^3} = \frac{x^3}{8}$

5. $\displaystyle \frac{3a^{3/2} \cdot a^{1/2}}{a^{-1}} = \frac{3a^2}{a^{-1}} = 3a^2 \cdot a = 3a^3$

6. $\displaystyle \frac{\sqrt{a\sqrt{b}}}{\sqrt[3]{ab}} = \frac{\sqrt{a} \cdot \sqrt[4]{b}}{\sqrt[3]{a} \cdot \sqrt[3]{b}} = a^{(\frac{1}{2}- \frac{1}{3})} \cdot b^{(\frac{1}{4}-\frac{1}{3})} = a^{\frac{1}{6}} \cdot b^{-\frac{1}{12}} = \frac{\sqrt[6]{a}}{\sqrt[12]{b}}$

</div>
