<div class="alert alert-warning" role="alert">
<h4 class="alert-heading">Problem 35-38</h4>

Evaluate the difference quotient for the given function. Simplify your answer.

35. $\displaystyle f(x) = 4+3x-x^2, \qquad \frac{f(3+h)-f(3)}{h}$

36. $\displaystyle f(x) = x^3, \qquad \frac{f(a+h)-f(a)}{h}$

37. $\displaystyle f(x) = \frac{1}{x}, \qquad \frac{f(x)-f(a)}{x-a}$

38. $\displaystyle f(x) = \sqrt{x+2}, \qquad \frac{f(x)-f(1)}{x-1}$

</div>

<div class="alert alert-success" role="alert">
<h4 class="alert-heading">Solution</h4>

**Problem 35**

$f(3+h) = 4+3 \cdot (3+h)-(3+h)^2 = 4-3h-h^2$

$f(3) = 4+3 \cdot 3-3^2=4$
    
$$ \frac{f(3+h)-f(3)}{h} = \frac{4-3h-h^2-4}{h} = \frac{-3h-h^2}{h} = -3-h $$

--------

**Problem 36**

$f(a+h) = (a+h)^3 = a^3 + 3a^2h + 3ah^2 + h^3$

$f(a) = a^3$

$$ \frac{f(a+h)-f(a)}{h} = \frac{a^3 + 3a^2h + 3ah^2 + h^3-a^3}{h} = 3a^2+3ah+h^2 $$

--------

**Problem 37**

$\displaystyle f(x) = \frac{1}{x}$

$\displaystyle f(a) = \frac{1}{a}$

$$ \frac{f(x)-f(a)}{x-a} = \frac{\frac{1}{x}-\frac{1}{a}}{x-a} = \frac{\frac{a-x}{xa}}{x-a} = -\frac{1}{ax}$$

--------

**Problem 38**

$f(x)=\sqrt{x+2}$

$f(1)=\sqrt{3}$

$$\frac{f(x)-f(1)}{x-1}=\frac{\sqrt{x+2}-\sqrt{3}}{x-1} $$

</div>

