<div class="alert alert-warning" role="alert">
<h4 class="alert-heading">Problem 23-30</h4>

Find a formula for the inverse of the function.

23. $\displaystyle f(x) = 1 - x^2, \quad x > 0$

24. $\displaystyle g(x) = x^2 - 2x, \quad x > 1$

25. $\displaystyle g(x) = 2 + \sqrt{x + 1}$

26. $\displaystyle h(x) = \frac{6 - 3x}{5x + 7}$

27. $\displaystyle y = e^{1-x}$

28. $\displaystyle y = 3 \ln (x - 2)$

29. $\displaystyle y = (2 + \sqrt[3]{x})^5$

30. $\displaystyle y = \frac{1 - e^{-x}}{1 + e^{-x}}$

</div>

<div class="alert alert-success" role="alert">
<h4 class="alert-heading">Solution</h4>



</div>

