<div class="alert alert-warning" role="alert">
<h4 class="alert-heading">Problem 6-7</h4>

The graph of $y = \sqrt{3x - x^2}$ is given. Use transformations to create a function whose graph is as shown.

</div>

![](_media/fig4.png ':size=80% :class=img-center')

<div class="alert alert-success" role="alert">
<h4 class="alert-heading">Solution</h4>

**Problem 6**

Shift $2$ units to the right and stretch vertically by a factor of $2$. Therefore, the transfered function is
$$y = 2\sqrt{3(x-2) - (x-2)^2} = 2\sqrt{-x^2+7x-10}$$

**Problem 7**

<!-- tabs:start -->

#### **Solution 1**

Shift $4$ units to the left and $1$ upward, then reflect about the $x$-axis. Therefore, the transfered function is
$$y = -(\sqrt{3(x+4) - (x+4)^2}+1) = -\sqrt{-x^2-5x-4}-1$$

#### **Solution 2**

Shift $1$ units to the right and $1$ upward, then reflect about the origin. Therefore, the transfered function is
$$y = -(\sqrt{3(-x-1) - (-x-1)^2}+1) = -\sqrt{-x^2-5x-4}-1$$

<!-- tabs:end -->

</div>

