<div class="alert alert-warning" role="alert">
<h4 class="alert-heading">Problem 41-44</h4>

Find $f \circ g \circ h$.

41. $\displaystyle f(x) = 3x-2, \quad g(x) = \sin x, \quad h(x) = x^2$

42. $\displaystyle f(x) = |x-4|, \quad g(x) = 2^x, \quad h(x) = \sqrt{x}$

43. $\displaystyle f(x) = \sqrt{x-3}, \quad g(x) = x^2, \quad h(x) = x^3+2$

44. $\displaystyle f(x) = \tan x, \quad g(x) = \frac{x}{x-1}, \quad h(x) = \sqrt[3]{x}$

</div>


<div class="alert alert-success" role="alert">
<h4 class="alert-heading">Solution</h4>

**Problem 41**

$$
\begin{aligned}
f \circ g \circ h &= f\Big(g\big(h(x)\big)\Big) \\
&= f\Big(g\big(x^2\big)\Big) \\
&= f\Big(\sin(x^2)\Big) \\
&= 3\sin(x^2)-2
\end{aligned}
$$

----

**Problem 42**

$$
\begin{aligned}
f \circ g \circ h &= f\Big(g\big(h(x)\big)\Big) \\
&= f\Big(g\big(\sqrt{x}\big)\Big) \\
&= f\Big(2^{\sqrt{x}}\Big) \\
&= |2^{\sqrt{x}}-4|
\end{aligned}
$$

----

**Problem 43**

$$
\begin{aligned}
f \circ g \circ h &= f\Big(g\big(h(x)\big)\Big) \\
&= f\Big(g\big(x^3+2\big)\Big) \\
&= f\Big(\big(x^3+2\big)^2\Big) = f\Big(x^6+4x^3+4\Big)\\
&= \sqrt{x^6+4x^3+4-3} = \sqrt{x^6+4x^3+1}
\end{aligned}
$$

----

**Problem 44**

$$
\begin{aligned}
f \circ g \circ h &= f\Big(g\big(h(x)\big)\Big) \\
&= f\Big(g\big(\sqrt[3]{x}\big)\Big) \\
&= f\Big(\frac{\sqrt[3]{x}}{\sqrt[3]{x}-1}\Big) \\
&= \tan \Big(\frac{\sqrt[3]{x}}{\sqrt[3]{x}-1}\Big)
\end{aligned}
$$

</div>

