<div class="alert alert-warning" role="alert">
<h4 class="alert-heading">Problem 55-56</h4>

Use the table to evaluate each expression.

<div style="text-align:center">
<table style="display:inline">
    <tr>
        <td style="background-color: #b5f4fc; font-weight: 600;"> x </td>
        <td>1</td><td>2</td><td>3</td><td>4</td><td>5</td><td>6</td>
    <tr>
    <tr>
        <td style="background-color: #b5f4fc; font-weight: 600;"> f(x) </td>
        <td>3</td><td>1</td><td>5</td><td>6</td><td>2</td><td>4</td>
    <tr>
    <tr>
        <td style="background-color: #b5f4fc; font-weight: 600;"> g(x) </td>
        <td>5</td><td>3</td><td>4</td><td>1</td><td>3</td><td>2</td>
    <tr>
</table>
</div>

55. (a) $f(g(3)) \quad$ (b) $g(f(2)) \quad$ (c) $(f \circ g)(5) \quad$ (d) $(g \circ f)(5)$

56. (a) $g(g(g(2))) \quad$ (b) $(f \circ f \circ f)(1) \quad$ (c) $(f \circ f \circ g)(1) \quad$ (d) $(g \circ f \circ g)(3)$

</div>


<div class="alert alert-success" role="alert">
<h4 class="alert-heading">Solution</h4>

**Problem 55**

- $f(g(3)) = f(4) = 6$

- $g(f(2)) = g(1) = 5$

- $(f \circ g)(5) = f(g(5)) = f(3) = 5$

- $(g \circ f)(5) = g(f(5)) = g(2) = 3$

----

**Problem 56**

- $g(g(g(2))) = g(g(3)) = g(4) = 1$

- $(f \circ f \circ f)(1) = f(f(f(1))) = f(f(3)) = f(5) = 2$

- $(f \circ f \circ g)(1) = f(f(g(1))) = f(f(5)) = f(2) = 1$

- $(g \circ f \circ g)(3) = g(f(g(3))) = g(f(4)) = g(6) = 2$

</div>

