<div class="alert alert-warning" role="alert">
<h4 class="alert-heading">Problem 13</h4>

Find a formula for a cubic function $f$ if $f(1) = 6$ and $f(-1) = f(0) = f(2) = 0$.

</div>

<div class="alert alert-success" role="alert">
<h4 class="alert-heading">Solution</h4>

From the equation $f(-1) = f(0) = f(2) = 0$, we know that $-1$, $0$, and $2$ are the real roots of the cubic equation $f(x)=0$. Therefore, we can express the cubic equation as 

$$f(x) = a(x+1)(x-0)(x-2)$$

Given that $f(1) = 6$, substituting $x = 1$ yields:

$$
\begin{align*}
a \cdot (1+1) \cdot (1-0) \cdot (1-2) &= 6 \\
-2a &= 6 \\ 
a &= -3
\end{align*}
$$

Thus, the formula for the cubic function $f$ is: 

$$
\begin{align*}
f(x) &= -3(x+1)x(x-2) \\
& = -3(x^2+x)(x-2) \\ 
& = -3(x^3-2x^2+x^2-2x) \\ 
& = -3(x^3-x^2-2x) \\ 
& = -3x^3+3x^2+6x
\end{align*}
$$

</div>

